Added With_functions section.

padlock.v
@@ -129,415 +129,566 @@ Inductive valid_code (c : code) : Prop :=
 
 
 
+Section Pure_theorems.
 
-
-Theorem same_digit_at_pos :
-  forall c d0 d1 p,
-    has_digit c d0 p ->
-      has_digit c d1 p ->
-        d0 = d1.
-Proof.
-  intros.
-  destruct c.
-  destruct p;
-    inversion H; subst;
-    inversion H0; subst;
-    reflexivity.
-Qed.
-
-Theorem three_different_as_all_pos (pr : position -> Prop) :
-  forall p0 p1 p2,
-    three_different_positions p0 p1 p2 ->
-      pr p0 -> pr p1 -> pr p2 ->
-        forall p, pr p.
-Proof.
-  intros.
-  destruct p;
-    destruct p0;
-    destruct p1;
-    destruct p2;
-    try auto;
-    try (
-      inversion H;
-      exfalso;
-      auto).
-Defined.
-
-Theorem always_one_of_three :
-  forall p p0 p1 p2,
-    three_different_positions p0 p1 p2 ->
-      p = p0 \/ p = p1 \/ p = p2.
-Proof.
-  intros.
-  inversion H; subst.
-  destruct p, p0;
-    try (left; reflexivity);
-    right;
-    destruct p1;
-    try (left; reflexivity);
-    right;
-    destruct p2;
-    try reflexivity;
-    try (exfalso; auto).
-Qed.
-
-Theorem code_012_condition_0 :
-  condition_0 (code_intro digit_0 digit_1 digit_2).
-Proof.
-  apply condition_0_intro with position_2 position_0 position_1.
-  - apply three_different_positions_intro;
-    intro H;
-    inversion H.
-  - apply match_at_position_intro with digit_2.
-    apply has_digit_2.
-    apply has_digit_2.
-  - apply invalid_digit_at_position_intro with digit_6.
-    * apply has_digit_0.
-    * intros pos1.
-      destruct pos1;
-        intro Hinv;
-        inversion Hinv.
-  - apply invalid_digit_at_position_intro with digit_8.
-    * apply has_digit_1.
-    * intros pos1.
-      destruct pos1;
-        intro Hinv;
-        inversion Hinv.
-Qed.
-
-Theorem code_012_condition_1 :
-  ~(condition_1 (code_intro digit_0 digit_1 digit_2)).
-Proof.
-  intro H.
-  inversion H; subst.
-  destruct p0.
-  - inversion H1; subst.
-    inversion H4; subst.
-    inversion H5.
-  - inversion H1; subst.
-    inversion H4; subst.
-    apply H6.
-    apply has_digit_1.
-  - inversion H1; subst.
-    inversion H4; subst.
-    inversion H5.
-Qed.
-
-Theorem code_012_is_not_valid :
-  ~(valid_code (code_intro digit_0 digit_1 digit_2)).
-Proof.
-  intro.
-  destruct H as [H0 H1 H2 H3 H4].
-  apply code_012_condition_1.
-  auto.
-Qed.
-
-Theorem invalid_8 :
-  forall c,
-    valid_code c ->
-      forall pos, ~(has_digit c digit_8 pos).
-Proof.
-  intros c H.
-  inversion H.
-  inversion H3; subst.
-  intros pos.
-  pose (H5 position_2) as H6.
-  inversion H6; subst.
-  inversion H7; subst.
-  apply H8.
-Qed.
-
-Theorem wrong_position_0_at_2 :
-  forall c,
-    valid_code c ->
-      has_digit c digit_0 position_0 \/ has_digit c digit_0 position_1.
-Proof.
-  intros.
-  inversion H.
-  inversion H3; subst.
-  inversion H4; subst.
-  assert (p0 <> position_0).
-  { intros Hinv.
-    subst.
-    inversion H7; subst.
-    inversion H10; subst.
-    apply (invalid_8 c H pos1).
-    apply H11. }
-  assert (p0 <> position_1).
-  { intros Hinv.
-    subst.
-    inversion H7; subst.
-    inversion H11; subst.
-    pose (H5 position_0) as H5_position_0.
-    inversion H5_position_0; subst.
-    inversion H14; subst.
-    apply (H15 pos1).
-    auto. }
-  assert (p0 = position_2).
-  { destruct p0.
-    - exfalso.
-      apply H10.
-      reflexivity.
-    - exfalso.
-      apply H11.
-      reflexivity.
-    - reflexivity. }
-  subst.
-  inversion H7; subst.
-  inversion H12; subst.
-  destruct pos1.
-  - left.
-    auto.
-  - right.
-    auto.
-  - exfalso.
-    apply H14.
-    auto.
-Qed.
-
-Theorem not_0_at_1 :
-  forall c,
-    valid_code c ->
-      ~(has_digit c digit_0 position_1).
-Proof.
-  intros c H Hinv.
-  inversion H.
-  inversion H2; subst.
-  assert (position_1 = p0 \/ position_1 = p1 \/ position_1 = p2) as Hchoice.
-  { apply always_one_of_three.
-    auto. }
-  destruct Hchoice as [Hc | [Hc | Hc]].
-  - subst.
-    inversion H6; subst.
-    inversion H9; subst.
-    auto.
-  - subst.
-    inversion H7; subst.
-    inversion H9; subst.
-    auto.
-  - subst.
-    inversion H8; subst.
-    inversion H9; subst.
-    apply (H10 position_1).
-    auto.
-Qed.
-
-Theorem correct_position_0_at_0 :
-  forall c,
-    valid_code c ->
-      has_digit c digit_0 position_0.
-Proof.
-  intros c H.
-  pose (wrong_position_0_at_2 c H) as H1.
-  destruct H1.
-  - auto.
-  - exfalso.
-    apply (not_0_at_1 c); auto.
-Qed.
-
-Theorem correct_position_2_at_2 :
-  forall c,
-    valid_code c ->
-      has_digit c digit_2 position_2.
-Proof.
-  intros c H.
-  inversion H.
-  inversion H0; subst.
-  destruct p0.
-  - inversion H6; subst.
-    inversion H9; subst.
-    assert (digit_6 = digit_0).
-    { apply same_digit_at_pos with c position_0; auto.
-      apply correct_position_0_at_0; auto. }
-    inversion H11.
-  - inversion H6; subst.
-    inversion H9; subst.
-    exfalso.
-    apply invalid_8 with c position_1; auto.
-  - inversion H6; subst.
-    inversion H9; subst.
-    auto.
-Qed.
-
-Theorem invalid_6 :
-  forall c,
-    valid_code c ->
-      forall pos, ~(has_digit c digit_6 pos).
-Proof.
-  intros c H.
-  inversion H.
-  inversion H2; subst.
-  destruct p2.
-  - inversion H8; subst.
-    inversion H9; subst.
-    exfalso.
-    apply (H10 position_2).
-    apply correct_position_2_at_2.
-    auto.
-  - inversion H8; subst.
-    inversion H9; subst.
-    exfalso.
-    apply (H10 position_0).
-    apply correct_position_0_at_0.
-    auto.
-  - inversion H8; subst.
-    inversion H9; subst.
-    apply H10.
-Qed.
-
-Theorem correct_position_4_at_1 :
-  forall c,
-    valid_code c ->
-      has_digit c digit_4 position_1.
-Proof.
-  intros c H.
-  inversion H.
-  inversion H1; subst.
-  destruct p0.
-  - exfalso.
-    inversion H6; subst.
-    inversion H9; subst.
-    apply invalid_6 with c pos1; auto.
-  - inversion H6; subst.
-    inversion H9; subst.
-    destruct pos1.
-    * assert (digit_1 = digit_0).
-      { apply same_digit_at_pos with c position_0.
-        - auto.
-        - apply correct_position_0_at_0.
-          auto. }
-      inversion H12.
-    * exfalso.
-      auto.
-    * assert (digit_1 = digit_2).
-      { apply same_digit_at_pos with c position_2.
-        - auto.
-        - apply correct_position_2_at_2.
-          auto. }
-      inversion H12.
-  - inversion H6; subst.
-    inversion H9; subst.
-    destruct pos1.
-    * assert (digit_4 = digit_0).
-      { apply same_digit_at_pos with c position_0.
-        - auto.
-        - apply correct_position_0_at_0.
-          auto. }
-      inversion H12.
-    * auto.
-    * assert (digit_4 = digit_2).
-      { apply same_digit_at_pos with c position_2.
-        - auto.
-        - apply correct_position_2_at_2.
-          auto. }
-      inversion H12.
-Qed.
-
-Definition code_042 :=
-  code_intro digit_0 digit_4 digit_2.
-
-Theorem only_valid_code_is_042 :
-  forall c,
-    valid_code c -> c = code_042.
-Proof.
-  intros c H.
-  assert (has_digit c digit_0 position_0) as Hd0.
-  { apply correct_position_0_at_0; auto. }
-  assert (has_digit c digit_4 position_1) as Hd1.
-  { apply correct_position_4_at_1; auto. }
-  assert (has_digit c digit_2 position_2) as Hd2.
-  { apply correct_position_2_at_2; auto. }
-  destruct c.
-  inversion Hd0; subst.
-  inversion Hd1; subst.
-  inversion Hd2; subst.
-  reflexivity.
-Qed.
-
-Theorem code_042_is_valid :
-  valid_code code_042.
-Proof.
-  apply valid_code_intro.
-  - apply condition_0_intro with position_2 position_0 position_1.
-    + apply three_different_positions_intro;
-      intro H;
-      inversion H.
-    + apply match_at_position_intro with digit_2.
-      * apply has_digit_2.
-      * apply has_digit_2.
-    + apply invalid_digit_at_position_intro with digit_6.
-      * apply has_digit_0.
-      * intros p H.
-        inversion H.
-    + apply invalid_digit_at_position_intro with digit_8.
-      * apply has_digit_1.
-      * intros p H.
-        inversion H.
-  - apply condition_1_intro with position_2 position_0 position_1.
-    + apply three_different_positions_intro;
-      intro H;
-      inversion H.
-    + apply wrong_position_intro with digit_4 position_1.
-      * apply has_digit_2.
-      * apply has_digit_1.
-      * intro H.
-        inversion H.
-    + apply invalid_digit_at_position_intro with digit_6.
-      * apply has_digit_0.
-      * intros pos1 H.
-        inversion H.
-    + apply invalid_digit_at_position_intro with digit_1.
-      * apply has_digit_1.
-      * intros pos1 H.
-        inversion H.
-  - apply condition_2_intro with position_0 position_1 position_2.
-    + apply three_different_positions_intro;
-      intro H;
-      inversion H.
-    + apply wrong_position_intro with digit_2 position_2.
-      * apply has_digit_0.
-      * apply has_digit_2.
-      * intros H.
-        inversion H.
-    + apply wrong_position_intro with digit_0 position_0.
-      * apply has_digit_1.
-      * apply has_digit_0.
-      * intro H.
-        inversion H.
-    + apply invalid_digit_at_position_intro with digit_6.
-      * apply has_digit_2.
-      * intros pos1 H.
-        inversion H.
-  - apply condition_3_intro.
+  Theorem same_digit_at_pos :
+    forall c d0 d1 p,
+      has_digit c d0 p ->
+        has_digit c d1 p ->
+          d0 = d1.
+  Proof.
     intros.
-    destruct pos.
-    + apply invalid_digit_at_position_intro with digit_7.
-      * apply has_digit_0.
-      * intros pos1 H.
-        inversion H.
-    + apply invalid_digit_at_position_intro with digit_3.
-      * apply has_digit_1.
-      * intros pos1 H.
-        inversion H.
-    + apply invalid_digit_at_position_intro with digit_8.
-      * apply has_digit_2.
-      * intros pos1 H.
-        inversion H.
-  - apply condition_4_intro with position_2 position_0 position_1.
-    + apply three_different_positions_intro;
+    destruct c.
+    destruct p;
+      inversion H; subst;
+      inversion H0; subst;
+      reflexivity.
+  Qed.
+
+  Theorem three_different_as_all_pos (pr : position -> Prop) :
+    forall p0 p1 p2,
+      three_different_positions p0 p1 p2 ->
+        pr p0 -> pr p1 -> pr p2 ->
+          forall p, pr p.
+  Proof.
+    intros.
+    destruct p;
+      destruct p0;
+      destruct p1;
+      destruct p2;
+      try auto;
+      try (
+        inversion H;
+        exfalso;
+        auto).
+  Defined.
+
+  Theorem always_one_of_three :
+    forall p p0 p1 p2,
+      three_different_positions p0 p1 p2 ->
+        p = p0 \/ p = p1 \/ p = p2.
+  Proof.
+    intros.
+    inversion H; subst.
+    destruct p, p0;
+      try (left; reflexivity);
+      right;
+      destruct p1;
+      try (left; reflexivity);
+      right;
+      destruct p2;
+      try reflexivity;
+      try (exfalso; auto).
+  Qed.
+
+  Theorem code_012_condition_0 :
+    condition_0 (code_intro digit_0 digit_1 digit_2).
+  Proof.
+    apply condition_0_intro with position_2 position_0 position_1.
+    - apply three_different_positions_intro;
       intro H;
       inversion H.
-    + apply wrong_position_intro with digit_0 position_0.
-      * apply has_digit_2.
+    - apply match_at_position_intro with digit_2.
+      apply has_digit_2.
+      apply has_digit_2.
+    - apply invalid_digit_at_position_intro with digit_6.
       * apply has_digit_0.
-      * intros H.
-        inversion H.
-    + apply invalid_digit_at_position_intro with digit_8.
-      * apply has_digit_0.
-      * intros pos1 H.
-        inversion H.
-    + apply invalid_digit_at_position_intro with digit_7.
+      * intros pos1.
+        destruct pos1;
+          intro Hinv;
+          inversion Hinv.
+    - apply invalid_digit_at_position_intro with digit_8.
       * apply has_digit_1.
-      * intros pos1 H.
+      * intros pos1.
+        destruct pos1;
+          intro Hinv;
+          inversion Hinv.
+  Qed.
+
+  Theorem code_012_condition_1 :
+    ~(condition_1 (code_intro digit_0 digit_1 digit_2)).
+  Proof.
+    intro H.
+    inversion H; subst.
+    destruct p0.
+    - inversion H1; subst.
+      inversion H4; subst.
+      inversion H5.
+    - inversion H1; subst.
+      inversion H4; subst.
+      apply H6.
+      apply has_digit_1.
+    - inversion H1; subst.
+      inversion H4; subst.
+      inversion H5.
+  Qed.
+
+  Theorem code_012_is_not_valid :
+    ~(valid_code (code_intro digit_0 digit_1 digit_2)).
+  Proof.
+    intro.
+    destruct H as [H0 H1 H2 H3 H4].
+    apply code_012_condition_1.
+    auto.
+  Qed.
+
+  Theorem invalid_8 :
+    forall c,
+      valid_code c ->
+        forall pos, ~(has_digit c digit_8 pos).
+  Proof.
+    intros c H.
+    inversion H.
+    inversion H3; subst.
+    intros pos.
+    pose (H5 position_2) as H6.
+    inversion H6; subst.
+    inversion H7; subst.
+    apply H8.
+  Qed.
+
+  Theorem wrong_position_0_at_2 :
+    forall c,
+      valid_code c ->
+        has_digit c digit_0 position_0 \/ has_digit c digit_0 position_1.
+  Proof.
+    intros.
+    inversion H.
+    inversion H3; subst.
+    inversion H4; subst.
+    assert (p0 <> position_0).
+    { intros Hinv.
+      subst.
+      inversion H7; subst.
+      inversion H10; subst.
+      apply (invalid_8 c H pos1).
+      apply H11. }
+    assert (p0 <> position_1).
+    { intros Hinv.
+      subst.
+      inversion H7; subst.
+      inversion H11; subst.
+      pose (H5 position_0) as H5_position_0.
+      inversion H5_position_0; subst.
+      inversion H14; subst.
+      apply (H15 pos1).
+      auto. }
+    assert (p0 = position_2).
+    { destruct p0.
+      - exfalso.
+        apply H10.
+        reflexivity.
+      - exfalso.
+        apply H11.
+        reflexivity.
+      - reflexivity. }
+    subst.
+    inversion H7; subst.
+    inversion H12; subst.
+    destruct pos1.
+    - left.
+      auto.
+    - right.
+      auto.
+    - exfalso.
+      apply H14.
+      auto.
+  Qed.
+
+  Theorem not_0_at_1 :
+    forall c,
+      valid_code c ->
+        ~(has_digit c digit_0 position_1).
+  Proof.
+    intros c H Hinv.
+    inversion H.
+    inversion H2; subst.
+    assert (position_1 = p0 \/ position_1 = p1 \/ position_1 = p2) as Hchoice.
+    { apply always_one_of_three.
+      auto. }
+    destruct Hchoice as [Hc | [Hc | Hc]].
+    - subst.
+      inversion H6; subst.
+      inversion H9; subst.
+      auto.
+    - subst.
+      inversion H7; subst.
+      inversion H9; subst.
+      auto.
+    - subst.
+      inversion H8; subst.
+      inversion H9; subst.
+      apply (H10 position_1).
+      auto.
+  Qed.
+
+  Theorem correct_position_0_at_0 :
+    forall c,
+      valid_code c ->
+        has_digit c digit_0 position_0.
+  Proof.
+    intros c H.
+    pose (wrong_position_0_at_2 c H) as H1.
+    destruct H1.
+    - auto.
+    - exfalso.
+      apply (not_0_at_1 c); auto.
+  Qed.
+
+  Theorem correct_position_2_at_2 :
+    forall c,
+      valid_code c ->
+        has_digit c digit_2 position_2.
+  Proof.
+    intros c H.
+    inversion H.
+    inversion H0; subst.
+    destruct p0.
+    - inversion H6; subst.
+      inversion H9; subst.
+      assert (digit_6 = digit_0).
+      { apply same_digit_at_pos with c position_0; auto.
+        apply correct_position_0_at_0; auto. }
+      inversion H11.
+    - inversion H6; subst.
+      inversion H9; subst.
+      exfalso.
+      apply invalid_8 with c position_1; auto.
+    - inversion H6; subst.
+      inversion H9; subst.
+      auto.
+  Qed.
+
+  Theorem invalid_6 :
+    forall c,
+      valid_code c ->
+        forall pos, ~(has_digit c digit_6 pos).
+  Proof.
+    intros c H.
+    inversion H.
+    inversion H2; subst.
+    destruct p2.
+    - inversion H8; subst.
+      inversion H9; subst.
+      exfalso.
+      apply (H10 position_2).
+      apply correct_position_2_at_2.
+      auto.
+    - inversion H8; subst.
+      inversion H9; subst.
+      exfalso.
+      apply (H10 position_0).
+      apply correct_position_0_at_0.
+      auto.
+    - inversion H8; subst.
+      inversion H9; subst.
+      apply H10.
+  Qed.
+
+  Theorem correct_position_4_at_1 :
+    forall c,
+      valid_code c ->
+        has_digit c digit_4 position_1.
+  Proof.
+    intros c H.
+    inversion H.
+    inversion H1; subst.
+    destruct p0.
+    - exfalso.
+      inversion H6; subst.
+      inversion H9; subst.
+      apply invalid_6 with c pos1; auto.
+    - inversion H6; subst.
+      inversion H9; subst.
+      destruct pos1.
+      * assert (digit_1 = digit_0).
+        { apply same_digit_at_pos with c position_0.
+          - auto.
+          - apply correct_position_0_at_0.
+            auto. }
+        inversion H12.
+      * exfalso.
+        auto.
+      * assert (digit_1 = digit_2).
+        { apply same_digit_at_pos with c position_2.
+          - auto.
+          - apply correct_position_2_at_2.
+            auto. }
+        inversion H12.
+    - inversion H6; subst.
+      inversion H9; subst.
+      destruct pos1.
+      * assert (digit_4 = digit_0).
+        { apply same_digit_at_pos with c position_0.
+          - auto.
+          - apply correct_position_0_at_0.
+            auto. }
+        inversion H12.
+      * auto.
+      * assert (digit_4 = digit_2).
+        { apply same_digit_at_pos with c position_2.
+          - auto.
+          - apply correct_position_2_at_2.
+            auto. }
+        inversion H12.
+  Qed.
+
+  Definition code_042 :=
+    code_intro digit_0 digit_4 digit_2.
+
+  Theorem only_valid_code_is_042 :
+    forall c,
+      valid_code c -> c = code_042.
+  Proof.
+    intros c H.
+    assert (has_digit c digit_0 position_0) as Hd0.
+    { apply correct_position_0_at_0; auto. }
+    assert (has_digit c digit_4 position_1) as Hd1.
+    { apply correct_position_4_at_1; auto. }
+    assert (has_digit c digit_2 position_2) as Hd2.
+    { apply correct_position_2_at_2; auto. }
+    destruct c.
+    inversion Hd0; subst.
+    inversion Hd1; subst.
+    inversion Hd2; subst.
+    reflexivity.
+  Qed.
+
+  Theorem code_042_is_valid :
+    valid_code code_042.
+  Proof.
+    apply valid_code_intro.
+    - apply condition_0_intro with position_2 position_0 position_1.
+      + apply three_different_positions_intro;
+        intro H;
         inversion H.
+      + apply match_at_position_intro with digit_2.
+        * apply has_digit_2.
+        * apply has_digit_2.
+      + apply invalid_digit_at_position_intro with digit_6.
+        * apply has_digit_0.
+        * intros p H.
+          inversion H.
+      + apply invalid_digit_at_position_intro with digit_8.
+        * apply has_digit_1.
+        * intros p H.
+          inversion H.
+    - apply condition_1_intro with position_2 position_0 position_1.
+      + apply three_different_positions_intro;
+        intro H;
+        inversion H.
+      + apply wrong_position_intro with digit_4 position_1.
+        * apply has_digit_2.
+        * apply has_digit_1.
+        * intro H.
+          inversion H.
+      + apply invalid_digit_at_position_intro with digit_6.
+        * apply has_digit_0.
+        * intros pos1 H.
+          inversion H.
+      + apply invalid_digit_at_position_intro with digit_1.
+        * apply has_digit_1.
+        * intros pos1 H.
+          inversion H.
+    - apply condition_2_intro with position_0 position_1 position_2.
+      + apply three_different_positions_intro;
+        intro H;
+        inversion H.
+      + apply wrong_position_intro with digit_2 position_2.
+        * apply has_digit_0.
+        * apply has_digit_2.
+        * intros H.
+          inversion H.
+      + apply wrong_position_intro with digit_0 position_0.
+        * apply has_digit_1.
+        * apply has_digit_0.
+        * intro H.
+          inversion H.
+      + apply invalid_digit_at_position_intro with digit_6.
+        * apply has_digit_2.
+        * intros pos1 H.
+          inversion H.
+    - apply condition_3_intro.
+      intros.
+      destruct pos.
+      + apply invalid_digit_at_position_intro with digit_7.
+        * apply has_digit_0.
+        * intros pos1 H.
+          inversion H.
+      + apply invalid_digit_at_position_intro with digit_3.
+        * apply has_digit_1.
+        * intros pos1 H.
+          inversion H.
+      + apply invalid_digit_at_position_intro with digit_8.
+        * apply has_digit_2.
+        * intros pos1 H.
+          inversion H.
+    - apply condition_4_intro with position_2 position_0 position_1.
+      + apply three_different_positions_intro;
+        intro H;
+        inversion H.
+      + apply wrong_position_intro with digit_0 position_0.
+        * apply has_digit_2.
+        * apply has_digit_0.
+        * intros H.
+          inversion H.
+      + apply invalid_digit_at_position_intro with digit_8.
+        * apply has_digit_0.
+        * intros pos1 H.
+          inversion H.
+      + apply invalid_digit_at_position_intro with digit_7.
+        * apply has_digit_1.
+        * intros pos1 H.
+          inversion H.
+  Qed.
+
+End Pure_theorems.
+
+Section With_functions.
+
+  Definition get_digit_at_pos (c : code) (p : position) :=
+    match c with
+    | code_intro d0 d1 d2 => match p with
+      | position_0 => d0
+      | position_1 => d1
+      | position_2 => d2
+      end
+    end.
+
+  Theorem get_digit_at_pos_correct :
+    forall c d p,
+      get_digit_at_pos c p = d <-> has_digit c d p.
+  Proof.
+    intros.
+    destruct c.
+    split.
+    + intro H.
+      destruct p; simpl in H; subst.
+      - apply has_digit_0.
+      - apply has_digit_1.
+      - apply has_digit_2.
+    + intro H.
+      destruct p;
+        simpl;
+        inversion H;
+        reflexivity.
+  Qed.
+
+  Definition digit_eq_bool (d0 d1 : digit) : bool :=
+    match d0, d1 with
+    | digit_0, digit_0 => true
+    | digit_1, digit_1 => true
+    | digit_2, digit_2 => true
+    | digit_3, digit_3 => true
+    | digit_4, digit_4 => true
+    | digit_5, digit_5 => true
+    | digit_6, digit_6 => true
+    | digit_7, digit_7 => true
+    | digit_8, digit_8 => true
+    | digit_9, digit_9 => true
+    | _, _ => false
+    end.
+
+  Theorem digit_eq_bool_correct :
+    forall d0 d1,
+      d0 = d1 <-> digit_eq_bool d0 d1 = true.
+  Proof.
+    split.
+    - intro H.
+      subst.
+      destruct d1;
+        reflexivity.
+    - intro H.
+      destruct d0, d1;
+        try reflexivity;
+        try inversion H.
+  Qed.
+
+  Definition match_at_position_bool (c0 c1 : code) (p : position) : bool :=
+    digit_eq_bool (get_digit_at_pos c0 p) (get_digit_at_pos c1 p).
+
+  Theorem match_at_position_bool_correct :
+    forall c0 c1 p,
+      match_at_position c0 c1 p <-> match_at_position_bool c0 c1 p = true.
+  Proof.
+    intros c0 c1 p.
+    unfold match_at_position_bool.
+    split.
+    - intro H.
+      apply digit_eq_bool_correct.
+      inversion H; subst.
+      apply get_digit_at_pos_correct in H0.
+      apply get_digit_at_pos_correct in H1.
+      subst.
+      auto.
+    - intro H.
+      apply digit_eq_bool_correct in H.
+      apply match_at_position_intro with (get_digit_at_pos c0 p).
+      + apply get_digit_at_pos_correct.
+        reflexivity.
+      + apply get_digit_at_pos_correct.
+        rewrite H.
+        reflexivity.
+  Qed.
+
+  Definition invalid_digit_at_position_bool (c0 c1 : code) (p : position) : bool :=
+    negb (digit_eq_bool (get_digit_at_pos c0 p) (get_digit_at_pos c1 position_0))
+    && negb (digit_eq_bool (get_digit_at_pos c0 p) (get_digit_at_pos c1 position_1))
+    && negb (digit_eq_bool (get_digit_at_pos c0 p) (get_digit_at_pos c1 position_2)).
+
+  Theorem invalid_digit_at_position_bool_correct :
+    forall c0 c1 p,
+      invalid_digit_at_position c0 c1 p <-> invalid_digit_at_position_bool c0 c1 p = true.
+  Proof.
+    intros.
+    split.
+    - intro H.
+      inversion H; subst.
+      unfold invalid_digit_at_position_bool.
+      apply get_digit_at_pos_correct in H0.
+      subst.
+      assert (forall pp, digit_eq_bool (get_digit_at_pos c0 p) (get_digit_at_pos c1 pp) = false) as Hpb.
+      { intro pp.
+        apply not_true_is_false.
+        intro Hinv.
+        apply H1 with pp.
+        apply digit_eq_bool_correct in Hinv.
+        apply get_digit_at_pos_correct.
+        rewrite <- Hinv.
+        reflexivity. }
+      rewrite (Hpb position_0).
+      rewrite (Hpb position_1).
+      rewrite (Hpb position_2).
+      reflexivity.
+    - intro H.
+      apply invalid_digit_at_position_intro with (get_digit_at_pos c0 p).
+      + apply get_digit_at_pos_correct.
+        reflexivity.
+      + intros pos1.
+        intro Hinv.
+        apply get_digit_at_pos_correct in Hinv.
+        unfold invalid_digit_at_position_bool in H.
+        rewrite <- Hinv in H.
+        apply andb_true_iff in H.
+        destruct H.
+        apply andb_true_iff in H.
+        destruct H.
+        apply negb_true_iff in H.
+        apply negb_true_iff in H0.
+        apply negb_true_iff in H1.
+        apply not_true_iff_false in H.
+        apply not_true_iff_false in H0.
+        apply not_true_iff_false in H1.
+        destruct pos1.
+        * apply H.
+          apply digit_eq_bool_correct.
+          reflexivity.
+        * apply H1.
+          apply digit_eq_bool_correct.
+          reflexivity.
+        * apply H0.
+          apply digit_eq_bool_correct.
+          reflexivity.
 Qed.
+
+End With_functions.
